\documentclass[12pt]{article}
\usepackage{latexsym, amsmath,amsfonts,amssymb}
\usepackage{xcolor}
\usepackage[margin=.75in]{geometry}
\usepackage{kpfonts}  %Changing the default fonts
\usepackage[T1]{fontenc}
\setlength{\parskip}{1.2ex} %space between paragraphs
\setlength{\parindent}{1em} %Paragraph indentation
\linespread{1.5} %spacing between lines
\pagestyle{empty}
\begin{document}
\begin{center}
\textbf{{\Large Three Essential Series for High School Students}}
\end{center}
\[\sum_{i=1}^{n}i=1+2+\cdots+n=\frac{n(n+1)}{2}\]\\
\textbf{Proof:} For any positive integer $n$ the equation $S=1+2+ \cdots +(n-1)+n$ can be written 
$S=n+(n-1)+\cdots+2+1$ as well. Adding the two equations together yields:
\[2S=\underbrace{(n+1)+(n+1)+\cdots+(n+1)+(n+1)}_\text{$n$ times}\]

This simplifies to $2S=n(n+1)$ or $S=\frac{n(n+1)}{2}$. Therefore,
$1+2+\cdots+(n-1)+n=\frac{n(n+1)}{2}$ from which it
follows $\sum_{i=1}^{n}i=\frac{n(n+1)}{2}$.\\

\[\sum_{i=1}^{n}i^2=1^2+2^2+\cdots + n^2=
\frac{n(n+1)(2n+1)}{6}\]

\noindent\textbf{Proof:} If $n=1$ then $\sum_{i=1}^{n}i^2=1^2=1=\frac{1(1+1)(2(1)+1)}{6}$ and the formula
is true. Now suppose the formula is true for some positive
integer $k$ and consider $\sum_{i=1}^{k+1}i^2=1^2+2^2+\cdots + k^2+(k+1)^2$. Since $\sum_{i=1}^{k+1}i^2=
\sum_{i=1}^{k}i^2+(k+1)^2$ the inductive hypothesis 
allows us to write this as $\frac{k(k+1)(2k+1)}{6}+(k+1)^2$.
This is equivalent to $\frac{k(k+1)(2k+1)+6(k+1)^2}{6}=
\frac{k(2k^2+3k+1)+6(k^2+2k+1)}{6}=
\frac{2k^3+3k^2+k+6k^2+12k+6)}{6}=
\frac{k^3+9k^2+13k+6)}{6} = 
\frac{(k^2+3k+2)(2k+3)}{6}=
\frac{(k+1)(k+2)(2(k+1)+1)}{6}$. Therefore $\sum_{i=1}^{k+1}i^2=\frac{(k+1)((k+1)+1)(2(k+1)+1)}{6}$
hence, by induction, it
follows $\sum_{i=1}^{n}i^2=1^2+2^2+
\cdots + n^2=\frac{n(n+1)(2n+1)}{6}$ for every 
positive integer $n$.\\

\[\sum_{i=1}^{n}i^3=1^3+2^3+\cdots + n^3=
\left(\frac{n(n+1)}{2}\right)^2\]

\noindent\textbf{Proof:} If $n=1$ then $\sum_{i=1}^{n}i^3=1^3=1=\left(\frac{1(1+1)}{2}\right)^2$ and 
the formula is true. Now suppose the formula is true for some 
positive integer $k$ and consider $\sum_{i=1}^{k+1}i^3=1^3+2^3+\cdots + k^3+(k+1)^3$. Since 
$\sum_{i=1}^{k+1}i^3=\sum_{i=1}^{k}i^3+(k+1)^3$
the inductive hypothesis allows us to write this as 
$\left(\frac{k(k+1)}{2}\right)^2+(k+1)^3$.
This is equivalent to $\frac{k^4+2k^3+k^2}{4}
+(k^3+3k^2+3k+1)=
\frac{k^4+2k^3+k^2+(4k^3+12k^2+12k+4)}{4}=
\frac{k^4+6k^3+13k^2+12k+4}{4}=
\left(\frac{(k+1)(k+2)}{2}\right)^2=
\left(\frac{(k+1)((k+1)+1)}{2}\right)^2$. Therefore,
$\sum_{i=1}^{k+1}i^3=\left(\frac{(k+1)((k+1)+1)}{2}\right)^2$ hence, by induction, it follows 
$\sum_{i=1}^{n}i^3=1^3+2^3+\cdots + n^3=
\left(\frac{n(n+1)}{2}\right)^2$ for every positive integer
$n$.
\end{document}